Makefile
@@ -24,7 +24,7 @@ tests:
 	coqc examples/Tests.v
 	cd examples/RedBlack; make clean && make
 	cd examples/stlc; make clean && make
-	cd examples/ifc-basic; make clean && make && coqc Driver.v
+	cd examples/ifc-basic; make clean && make
 
 Makefile.coq: Make
 	coq_makefile -f Make -o Makefile.coq
